@prefix rdf: <http://www.w3.org/1999/02/22-rdf-syntax-ns#> .
@prefix rdfs: <http://www.w3.org/2000/01/rdf-schema#> .
@prefix owl: <http://www.w3.org/2002/07/owl#> .
@prefix xsd: <http://www.w3.org/2001/XMLSchema#> .
@prefix dqv: <http://www.w3.org/ns/dqv#> .
@prefix skos: <http://www.w3.org/2004/02/skos/core#> .
@prefix oqo: <http://purl.org/oqo/> .
@prefix oqo-model: <http://purl.org/oqo/model#> .

<http://purl.org/oqo> a owl:Ontology ;
    rdfs:comment "Ontology Quality Ontology" ;
    owl:versionIRI <http://purl.org/oqo/version/1.0> .

oqo-model:Metric a owl:Class ;
    rdfs:label "Metric" ;
    rdfs:comment "A sample metric." .

oqo-model:ontology-set-metadata a owl:Class ;
    rdfs:label "Ontology Set Metadata"@en ;
    rdfs:comment "Metadata describing the results of processing over a set of ontologies"@en ;

oqo:ontology-count a owl:DatatypeProperty;
    rdfs:domain oqo-model:ontology-set-metadata ;
    rdfs:range xsd:integer ;
    rdfs:label "Ontology count"@en .

oqo:failed-count a owl:DatatypeProperty ;
    rdfs:domain oqo-model:ontology-set-metadata ;
    rdfs:range xsd:integer ;
    rdfs:label "Failed count"@en .

oqo-model:abox-axiom-count a dqv:Metric ;
    skos:prefLabel "ABox Axiom Count"@en ;
    skos:definition "Number of axioms in the ABox"@en ;
    dqv:expectedDataType xsd:integer ;
    dqv:inDimension oqo:ontology-size .

oqo-model:annotation-property-count a dqv:Metric ;
    skos:prefLabel "Annotation Property Count"@en ;
    skos:definition "Number of annotation properties"@en ;
    dqv:expectedDataType xsd:integer ;
    dqv:inDimension oqo:ontology-size .

oqo-model:assert-n-subclass-avg a dqv:Metric ;
    skos:prefLabel "Average Asserted Subclasses"@en ;
    skos:definition "Average number of (asserted) subclasses per class"@en ;
    dqv:expectedDataType xsd:double ;
    dqv:inDimension oqo:ontology-size .

oqo-model:assert-n-superclass-avg a dqv:Metric ;
    skos:prefLabel "Average Asserted Superclasses"@en ;
    skos:definition "Average number of (asserted) superclasses per class"@en ;
    dqv:expectedDataType xsd:double ;
    dqv:inDimension oqo:ontology-size .

oqo-model:ax-complexrhs-count a dqv:Metric ;
    skos:prefLabel "Complex RHS Axiom Count"@en ;
    skos:definition "Number of axioms with a complex right hand side"@en ;
    dqv:expectedDataType xsd:integer ;
    dqv:inDimension oqo:ontology-size .

oqo-model:axiom-count a dqv:Metric ;
    skos:prefLabel "Total Axiom Count"@en ;
    skos:definition "Number of axioms"@en ;
    dqv:expectedDataType xsd:integer ;
    dqv:inDimension oqo:ontology-size .


oqo-model:axiom-length-max a dqv:Metric ;
    skos:prefLabel "Max Axiom Length"@en ;
    skos:definition "Longest axiom in terms of number of entities used (including duplicate uses)."@en ;
    dqv:expectedDataType xsd:integer ;
    dqv:inDimension oqo:ontology-size .


oqo-model:axiom-type-count a dqv:Metric ;
    skos:prefLabel "Axiom Type Count"@en ;
    skos:definition "Number of axioms of a specific type, such as SubClassOf"@en ;
    dqv:expectedDataType xsd:string ;
    dqv:inDimension oqo:ontology-size .

oqo-model:axiom-types a dqv:Metric ;
    skos:prefLabel "Axiom Types Presence"@en ;
    skos:definition "Indicates the presence of an axiom type in the ontology."@en ;
    dqv:expectedDataType xsd:string ;
    dqv:inDimension oqo:ontology-size .

oqo-model:certain-cycle a dqv:Metric ;
    skos:prefLabel "Definite Cycle Detection"@en ;
    skos:definition "If true, there is a definite cycle in the ontology. If false, cyclicity is unknown (experimental)."@en ;
    dqv:expectedDataType xsd:boolean ;
    dqv:inDimension oqo:cycle-detection .

oqo-model:class-count a dqv:Metric ;
    skos:prefLabel "Class Count"@en ;
    skos:definition "Number of classes in the ontology"@en ;
    dqv:expectedDataType xsd:integer ;
    dqv:inDimension oqo:ontology-size .

oqo-model:class-sgl-subcl-count a dqv:Metric ;
    skos:prefLabel "Superclass with Multiple Subclasses Count"@en ;
    skos:definition "Number of super-classes which have more than one subclass."@en ;
    dqv:expectedDataType xsd:integer ;
    dqv:inDimension oqo:ontology-size .

oqo-model:constructs a dqv:Metric ;
    skos:prefLabel "Logical Constructs Used"@en ;
    skos:definition "Logical constructs used"@en ;
    dqv:expectedDataType xsd:string ;
    dqv:inDimension oqo:ontology-size .

oqo-model:dataproperty-count a dqv:Metric ;
    skos:prefLabel "Data Property Count"@en ;
    skos:definition "Number of distinct data properties."@en ;
    dqv:expectedDataType xsd:integer ;
    dqv:inDimension oqo:ontology-size .

oqo-model:datatypes-builtin a dqv:Metric ;
    skos:prefLabel "Built-in Datatypes Used"@en ;
    skos:definition "Datatypes used from the built-in datatype map (like XSD schema datatypes)."@en ;
    dqv:expectedDataType xsd:string ;
    dqv:inDimension oqo:ontology-size .

oqo-model:datatypes-count a dqv:Metric ;
    skos:prefLabel "Datatype Count"@en ;
    skos:definition "Total number of distinct datatypes."@en ;
    dqv:expectedDataType xsd:integer .
    dqv:inDimension oqo:ontology-size .

oqo-model:dt-builtin-count a dqv:Metric ;
    skos:prefLabel "Built-in Datatype Count"@en ;
    skos:definition "Total number of distinct built-in datatypes."@en ;
    dqv:expectedDataType xsd:integer ;
    dqv:inDimension oqo:ontology-size .

oqo-model:dt-notbuiltin-count a dqv:Metric ;
    skos:prefLabel "Custom Datatype Count"@en ;
    skos:definition "Total number of distinct custom (not built-in) datatypes."@en ;
    dqv:expectedDataType xsd:integer ;
    dqv:inDimension oqo:ontology-size .


oqo-model:gci-count a dqv:Metric ;
    skos:prefLabel "General Class Inclusion (GCI) Count"@en ;
    skos:definition "Total count of GCI axioms."@en ;
    dqv:expectedDataType xsd:integer ;
    dqv:inDimension oqo:ontology-size .

oqo-model:gci-hidden-count a dqv:Metric ;
    skos:prefLabel "Hidden GCI Count"@en ;
    skos:definition "Total count of hidden GCIs."@en ;
    dqv:expectedDataType xsd:integer ;
    dqv:inDimension oqo:ontology-size .

oqo-model:individual-count a dqv:Metric ;
    skos:prefLabel "Individual Count"@en ;
    skos:definition "Number of individuals."@en ;
    dqv:expectedDataType xsd:integer ;
    dqv:inDimension oqo:ontology-size .

oqo-model:instance-per-class-avg a dqv:Metric ;
    skos:prefLabel "Average Individuals per Class"@en ;
    skos:definition "Average number of individuals per class."@en ;
    dqv:expectedDataType xsd:double ;
    dqv:inDimension oqo:ontology-size .

oqo-model:namespace-axiom-count a dqv:Metric ;
    skos:prefLabel "Namespace Axiom Count"@en ;
    skos:definition "Number of axioms using at least one term in a namespace."@en ;
    dqv:expectedDataType xsd:string ;
    dqv:inDimension oqo:ontology-size .

oqo-model:namespace-entity-count a dqv:Metric ;
    skos:prefLabel "Namespace Entity Count"@en ;
    skos:definition "Number of distinct entities used from a namespace."@en ;
    dqv:expectedDataType xsd:string ;
    dqv:inDimension oqo:ontology-size .

oqo-model:logical-axiom-count a dqv:Metric ;
    skos:prefLabel "Logical Axiom Count"@en ;
    skos:definition "Number of logical axioms in ontology"@en ;
    dqv:expectedDataType xsd:integer ;
    dqv:inDimension oqo:ontology-size .

oqo-model:most-freq-concept a dqv:Metric ;
    skos:prefLabel "Most Frequent Concept"@en ;
    skos:definition "Most frequently used class."@en ;
    dqv:expectedDataType xsd:string ;
    dqv:inDimension oqo:ontology-size .

oqo-model:multiple-inheritance-count a dqv:Metric ;
    skos:prefLabel "Multiple Inheritance Class Count"@en ;
    skos:definition "Number of classes with multiple inheritance."@en ;
    dqv:expectedDataType xsd:integer ;
    dqv:inDimension oqo:ontology-size .

oqo-model:named-supercl-count-max a dqv:Metric ;
    skos:prefLabel "Max Named Superclasses"@en ;
    skos:definition "Maximum number of named superclasses."@en ;
    dqv:expectedDataType xsd:integer ;
    dqv:inDimension oqo:ontology-size .

oqo-model:obj-property-count a dqv:Metric ;
    skos:prefLabel "Object Property Count"@en ;
    skos:definition "Number of object properties."@en ;
    dqv:expectedDataType xsd:integer ;
    dqv:inDimension oqo:ontology-size .

oqo-model:ontology-anno-count a dqv:Metric ;
    skos:prefLabel "Ontology Annotation Count"@en ;
    skos:definition "Number of ontology annotations."@en ;
    dqv:expectedDataType xsd:integer ;
    dqv:inDimension oqo:ontology-size .

oqo-model:ontology-id a dqv:Metric ;
    skos:prefLabel "Ontology ID"@en ;
    skos:definition "The ontology id."@en ;
    dqv:expectedDataType xsd:anyURI ;
    dqv:inDimension oqo:ontology-metadata-dimension .

oqo-model:owl2-dl a dqv:Metric ;
    skos:prefLabel "OWL2 DL Compliance"@en ;
    skos:definition "Does the ontology correspond to the OWL2 DL profile?"@en ;
    dqv:expectedDataType xsd:boolean ;
    dqv:inDimension oqo:owl2-compliance .

oqo-model:owl2-el a dqv:Metric ;
    skos:prefLabel "OWL2 EL Compliance"@en ;
    skos:definition "Does the ontology correspond to the OWL2 EL profile?"@en ;
    dqv:expectedDataType xsd:boolean ;
    dqv:inDimension oqo:owl2-compliance .

oqo-model:owl2-ql a dqv:Metric ;
    skos:prefLabel "OWL2 QL Compliance"@en ;
    skos:definition "Does the ontology correspond to the OWL2 QL profile?"@en ;
    dqv:expectedDataType xsd:boolean ;
    dqv:inDimension oqo:owl2-compliance .

oqo-model:owl2-rl a dqv:Metric ;
    skos:prefLabel "OWL2 RL Compliance"@en ;
    skos:definition "Does the ontology correspond to the OWL2 RL profile?"@en ;
    dqv:expectedDataType xsd:boolean ;
    dqv:inDimension oqo:owl2-compliance .

oqo-model:owl2 a dqv:Metric ;
    skos:prefLabel "OWL2 Full Compliance"@en ;
    skos:definition "Does the ontology correspond to the OWL2 Full profile?"@en ;
    dqv:expectedDataType xsd:boolean ;
    dqv:inDimension oqo:owl2-compliance .

oqo-model:owl2dl-profile-violation a dqv:Metric ;
    skos:prefLabel "OWL2 DL Profile Violation Count"@en ;
    skos:definition "Counts of OWL2 DL profile violations."@en ;
    dqv:expectedDataType xsd:string ;
    dqv:inDimension oqo:owl2-compliance .

oqo-model:rbox-axiom-count a dqv:Metric ;
    skos:prefLabel "RBOX Axiom Count"@en ;
    skos:definition "How many axioms in the RBOX?"@en ;
    dqv:expectedDataType xsd:integer ;
    dqv:inDimension oqo:ontology-size .

oqo-model:rdfs a dqv:Metric ;
    skos:prefLabel "RDFS Compliance"@en ;
    skos:definition "Does the ontology correspond to the RDFS profile?"@en ;
    dqv:expectedDataType xsd:boolean ;
    dqv:inDimension oqo:rdfs-compliance .

oqo-model:rule-count a dqv:Metric ;
    skos:prefLabel "Rule Count"@en ;
    skos:definition "Number of SWRL rules used."@en ;
    dqv:expectedDataType xsd:integer ;
    dqv:inDimension oqo:ontology-size .


oqo-model:signature-entity-count a dqv:Metric ;
    skos:prefLabel "Signature Entity Count"@en ;
    skos:definition "Total number of entities in signature, including classes and individuals."@en ;
    dqv:expectedDataType xsd:integer ;
    dqv:inDimension oqo:ontology-size .

oqo-model:syntax a dqv:Metric ;
    skos:prefLabel "Ontology Syntax"@en ;
    skos:definition "What serialisation is used for the ontology?"@en ;
    dqv:expectedDataType xsd:string ;
    dqv:inDimension oqo:ontology-representation;

oqo-model:tautology-count a dqv:Metric ;
    skos:prefLabel "Tautology Count"@en ;
    skos:definition "Number of tautological axioms."@en ;
    dqv:expectedDataType xsd:integer ;
    dqv:inDimension oqo:ontology-size .


oqo-model:tbox-axiom-count a dqv:Metric ;
    skos:prefLabel "TBOX Axiom Count"@en ;
    skos:definition "Number of TBOX axioms (without RBOX)."@en ;
    dqv:expectedDataType xsd:integer ;
    dqv:inDimension oqo:ontology-size .


oqo-model:tbox-nominals a dqv:Metric ;
    skos:prefLabel "TBOX Nominals Count"@en ;
    skos:definition "Number of TBOX axioms with nominals."@en ;
    dqv:expectedDataType xsd:boolean ;
    dqv:inDimension oqo:ontology-size .


oqo-model:tboxrbox-axiom-count a dqv:Metric ;
    skos:prefLabel "TBOX+RBOX Axiom Count"@en ;
    skos:definition "Number of TBOX axioms (with RBOX)."@en ;
    dqv:expectedDataType xsd:integer ;
    dqv:inDimension oqo:ontology-size .


oqo-model:undecl-entity-count a dqv:Metric ;
    skos:prefLabel "Undeclared Entity Count"@en ;
    skos:definition "Number of undeclared entities."@en ;
    dqv:expectedDataType xsd:integer ;
    dqv:inDimension oqo:ontology-size .




oqo:owl2-compliance a dqv:Dimension ;
    skos:prefLabel "Profile Compliance"@en ;
    skos:definition "Dimension measuring the compliance of the ontology with different OWL2 profiles (DL, EL, QL, RL, Full)."@en ;
    dqv:inCategory oqo:compliance .

oqo:ontology-size a dqv:Dimension ;
    skos:prefLabel "Ontology Size"@en ;
    skos:definition "Measures the size of the ontology in terms of axioms and entities."@en ;
    dqv:inCategory oqo:structuralQuality .

oqo:cycle-detection a dqv:Dimension ;
    skos:prefLabel "Cycle Detection"@en ;
    skos:definition "Dimension that measures the presence or absence of cycles in the ontology."@en ;
    dqv:inCategory oqo:structuralQuality .

oqo:ontology-metadata-dimension a dqv:Dimension ;
    skos:prefLabel "Ontology Metadata"@en ;
    skos:definition "Dimension that measures key metadata characteristics of the ontology, such as its ID."@en ;
    dqv:inCategory oqo:ontologyMetadata .

oqo:rdfs-compliance a dqv:Dimension ;
    skos:prefLabel "RDFS Compliance"@en ;
    skos:definition "Dimension measuring the compliance of the ontology with the RDFS profile."@en ;
    dqv:inCategory oqo:compliance .

oqo:ontology-representation a dqv:Dimension ;
    skos:prefLabel "Ontology Representation"@en ;
    skos:definition "Dimension measuring the representation format of the ontology, including serialization and syntax."@en ;
    dqv:inCategory oqo:representation.



oqo:ontology-metadata a dqv:Category ;
    skos:prefLabel "Ontology Metadata"@en ;
    skos:definition "Category that groups dimensions related to the metadata of the ontology, such as its ID and other identifying features."@en .

oqo:compliance a dqv:Category ;
    skos:prefLabel "Compliance"@en ;
    skos:definition "Category that groups dimensions measuring the ontology's compliance."@en ;

oqo:structural-quality a dqv:Category ;
    skos:prefLabel "Structural Quality"@en ;
    skos:definition "Category that groups dimensions measuring size and structural complexity of an ontology. This category includes aspects like the number of axioms, entities, and logical constructs in the ontology."@en ;

oqo:representation a dqv:Category ;
    skos:prefLabel "Ontology Representation"@en ;
    skos:definition "Category that groups dimensions related to the representation and structure of the ontology, including syntax and serialization."@en .
